Lean/Egg/Core/MVars/Collect.lean
@@ -1,0 +1,96 @@
+import Egg.Core.MVars.Basic
+import Egg.Core.MVars.Ambient
+import Lean
+
+open Lean Meta
+
+namespace Egg.MVars.CollectionM
+
+private structure State where
+  mvars  : MVars
+  active : Properties
+  amb    : Ambient
+
+private abbrev _root_.Egg.MVars.CollectionM := StateT CollectionM.State MetaM
+
+private nonrec def run (m : CollectionM Unit) (amb : Ambient) : MetaM MVars := do
+  let (_, state) ← m.run { mvars := {}, active := ∅, amb }
+  return state.mvars
+
+private def active : CollectionM Properties :=
+  return (← get).active
+
+private def amb : CollectionM Ambient :=
+  return (← get).amb
+
+private def withProperty (p : Property) (m : CollectionM α) : CollectionM α := do
+  let { active, .. } ← getModify fun s => { s with active := s.active.insert p }
+  let a ← m
+  modify ({ · with active })
+  return a
+
+private def collectMVar (mvar : MVarId) : CollectionM Unit := do
+  if (← amb).expr.contains mvar then return
+  let isTcInst ← Meta.isTCInstance (.mvar mvar)
+  modify fun s =>
+    let ps := s.active
+      |>.insertIf isTcInst .isTcInst
+      |>.insertIf (!s.active.containsErased) .inTarget
+    { s with mvars := s.mvars.insertExpr mvar ps }
+
+private def collectLMVar (lmvar : LMVarId) : CollectionM Unit := do
+  if (← amb).lvl.contains lmvar then return
+  modify fun s =>
+    let ps := s.active.insertIf (!s.active.containsErased) .inTarget
+    { s with mvars := s.mvars.insertLevel lmvar ps }
+
+private def collectLevel (lvl : Level) : CollectionM Unit := do
+  for lmvar in lvl.collectMVars do collectLMVar lmvar
+
+private def collectLevels (lvls : List Level) : CollectionM Unit := do
+  for lvl in lvls do collectLevel lvl
+
+private partial def collect (e : Expr) : CollectionM Unit := do
+  -- We check if `e` is an ambient mvar here (as opposed to only checking for ambient mvars in
+  -- `collect{L}MVar`), in order to avoid looking at its type in that case.
+  if ← isAmbientMVar e then
+    return
+  else if ← Meta.isTCInstance e then
+    withProperty .inTcInstTerm do core e
+    withProperty .inErasedTcInst do core (← inferType e)
+  else if ← Meta.isProof e then
+    withProperty .inProofTerm   do core e
+    withProperty .inErasedProof do core (← inferType e)
+  else
+    core e
+where
+  isAmbientMVar (e : Expr) : CollectionM Bool := do
+    let .mvar m := e | return false
+    return (← amb).expr.contains m
+
+  core (e : Expr) : CollectionM Unit := do
+    unless e.hasMVar do return
+    match e with
+    | .mvar id      => collectMVar id
+    | .const _ lvls => collectLevels lvls
+    | .sort lvl     => collectLevel lvl
+    | .app fn arg   => coreRec fn; coreRec arg
+    | .forallE _ ty b _ | .lam _ ty b _ =>
+      coreRec ty
+      withLocalDecl .anonymous .default ty fun fvar => coreRec (b.instantiate #[fvar])
+    | .letE .. | .mdata .. | .proj .. =>
+      panic! "'Egg.MVars.CollectionM.collect.core' received non-normalized expression"
+    -- Note: This should not be reachable as we check whether `e` contains mvars at the beginning.
+    | _ => return
+
+  -- When `core` performs a recursive call, we choose whether to call `core` or `collect` depending
+  -- on whether there are any active properties. If there already is an active property, then we
+  -- don't want to consider additional properties and simply call `core` again. If there are no
+  -- active properties yet, then we call `collect` which checks whether a property is satisfied.
+  coreRec (e : Expr) : CollectionM Unit := do
+    if (← active).isEmpty then collect e else core e
+
+end CollectionM
+
+def collect (e : Expr) (amb : Ambient) : MetaM MVars :=
+  CollectionM.collect e |>.run amb
