Lean/Egg/Core/Request/Synth.lean
@@ -1,0 +1,6 @@
+import Egg
+import Lean
+open Lean
+
+def isSynthable? (s : String) : MetaM Bool := do
+  sorry
