Lean/Egg/Tests/MVars Properties.lean
@@ -1,0 +1,67 @@
+import Egg
+open scoped Egg
+
+egg_no_defeq
+set_option egg.builtins false
+set_option egg.genTcProjRws false
+set_option trace.egg.rewrites true
+
+/--
+info: [egg.rewrites] Rewrites
+  [egg.rewrites] Basic (1)
+    [egg.rewrites] #0(⇔): h
+      [egg.rewrites] ?x = ?x
+      [egg.rewrites] LHS MVars
+          [?x: [.inTarget]]
+      [egg.rewrites] RHS MVars
+          [?x: [.inTarget]]
+  [egg.rewrites] Tagged (0)
+  [egg.rewrites] Builtin (0)
+  [egg.rewrites] Derived (0)
+  [egg.rewrites] Definitional
+  [egg.rewrites] Hypotheses (0)
+  [egg.rewrites] Pruned (0)
+-/
+#guard_msgs(info) in
+example (h : ∀ x : Nat, x = x) : true = true := by
+  egg [h]
+
+/--
+info: [egg.rewrites] Rewrites
+  [egg.rewrites] Basic (1)
+    [egg.rewrites] #0(⇒): h
+      [egg.rewrites] f ?x = ?x
+      [egg.rewrites] LHS MVars
+          [?x: [.inTarget], ?α: [.inTarget]]
+      [egg.rewrites] RHS MVars
+          [?x: [.inTarget]]
+  [egg.rewrites] Tagged (0)
+  [egg.rewrites] Builtin (0)
+  [egg.rewrites] Derived (0)
+  [egg.rewrites] Definitional
+  [egg.rewrites] Hypotheses (0)
+  [egg.rewrites] Pruned (0)
+-/
+#guard_msgs(info) in
+example (f : {α : Type} → α → α) (h : ∀ α (x : α), f x = x) : true = true := by
+  egg [h]
+
+/--
+info: [egg.rewrites] Rewrites
+  [egg.rewrites] Basic (1)
+    [egg.rewrites] #0(⇒): h
+      [egg.rewrites] ?x + ?x = ?x
+      [egg.rewrites] LHS MVars
+          [?x: [.inTarget], ?inst✝: [.inTcInstTerm, .isTcInst, .inTarget]]
+      [egg.rewrites] RHS MVars
+          [?x: [.inTarget]]
+  [egg.rewrites] Tagged (0)
+  [egg.rewrites] Builtin (0)
+  [egg.rewrites] Derived (0)
+  [egg.rewrites] Definitional
+  [egg.rewrites] Hypotheses (0)
+  [egg.rewrites] Pruned (0)
+-/
+#guard_msgs(info) in
+example (h : ∀ [Add α] (x : α), x + x = x) : true = true := by
+  egg [h]
